revise

src/Minimal.DICE.fst
@@ -24,7 +24,7 @@ module HS  = FStar.HyperStack
 module HST = FStar.HyperStack.ST
 module IB  = LowStar.ImmutableBuffer
 
-inline_for_extraction noextract
+unfold inline_for_extraction noextract
 let dice_hash (alg: dice_alg): hash_st alg =
   match alg with
   | SHA2_256 -> SHA2.hash_256
@@ -32,7 +32,7 @@ let dice_hash (alg: dice_alg): hash_st alg =
   | SHA2_512 -> SHA2.hash_512
   | SHA1     -> SHA1.legacy_hash
 
-inline_for_extraction noextract
+unfold inline_for_extraction noextract
 let dice_hmac (alg: dice_alg): HMAC.compute_st alg =
   match alg with
   | SHA2_256 -> HMAC.compute_sha2_256
@@ -40,89 +40,11 @@ let dice_hmac (alg: dice_alg): HMAC.compute_st alg =
   | SHA2_512 -> HMAC.compute_sha2_512
   | SHA1     -> HMAC.legacy_compute_sha1
 
-/// compute digest of `uds`
-inline_for_extraction
-let compute_uDigest
-  (uDigest: B.buffer uint8{B.length uDigest == hash_length alg})
-  (uds: B.buffer uint8{B.length uds == v uds_length})
-: HST.StackInline unit
-  (requires fun h ->
-    B.all_live h [B.buf uDigest
-                 ;B.buf uds] /\
-    B.all_disjoint [B.loc_buffer uDigest
-                   ;B.loc_buffer uds])
-  (ensures  fun h0 _ h1 ->
-    B.modifies (B.loc_buffer uDigest) h0 h1 /\
-    B.as_seq h1 uDigest
-      == Spec.Agile.Hash.hash alg (B.as_seq h0 uds))
-=
-  dice_hash alg
-    uds
-    uds_length
-    uDigest
-
-/// compute measurement of RIoT firmware
-inline_for_extraction
-let compute_rDigest
-  (rDigest: B.buffer uint8{B.length rDigest == hash_length alg})
-  (riot_size: riot_size_t)
-  (riot_binary: B.buffer uint8 {B.length riot_binary == v riot_size})
-: HST.StackInline unit
-  (requires fun h ->
-    B.all_live h [B.buf riot_binary
-                 ;B.buf rDigest] /\
-    B.all_disjoint [B.loc_buffer riot_binary
-                   ;B.loc_buffer rDigest])
-  (ensures  fun h0 _ h1 ->
-    B.live h1 riot_binary /\
-    B.modifies (B.loc_buffer rDigest) h0 h1 /\
-    B.as_seq h1 rDigest
-      == Spec.Agile.Hash.hash alg (B.as_seq h0 riot_binary))
-=
-  dice_hash alg
-    riot_binary
-    riot_size
-    rDigest
-
-/// Compute `cdi`
-inline_for_extraction
-let compute_cdi
-  (cdi: B.buffer uint8{B.length cdi == v cdi_length /\ B.freeable cdi})
-  (uDigest: B.buffer uint8{B.length uDigest == hash_length alg})
-  (rDigest: B.buffer uint8{B.length rDigest == hash_length alg})
-: HST.StackInline unit
-  (requires fun h ->
-      B.all_live h [B.buf cdi
-                   ;B.buf uDigest
-                   ;B.buf rDigest]
-    /\ B.all_disjoint [B.loc_buffer cdi
-                     ;B.loc_buffer uDigest
-                     ;B.loc_buffer rDigest])
-  (ensures  fun h0 _ h1 ->
-    B.modifies (B.loc_buffer cdi) h0 h1 /\
-    B.as_seq h1 cdi
-      == Spec.Agile.HMAC.hmac alg (B.as_seq h0 uDigest) (B.as_seq h0 rDigest))
-=
-  (**)let h = HST.get() in
-  (**)assert (Spec.Agile.HMAC.keysized alg (Seq.length (B.as_seq h uDigest)));
-  dice_hmac alg
-    cdi
-    uDigest (hash_len alg)
-    rDigest (hash_len alg)
-
-///
-/// if we treat `riot_t` as a argument of `dice_main`, then it will be allocated before we call `initialize ()` allocate `uds` and `cdi`, hence we cannot derive the disjointness between `riot.binary` and `uds` or `cdi`
-///
-/// Since we cannot directly allocate a buffer and "load" RIoT in F*, I will add a `riot_t` into hardware `state` and allocate it in the heap rather then on a stack.
-///
-/// DICE procedure on a stack
-/// It has `Stack` effect, which can only do local stack allocations.
-/// FIXME: Will stack be "clean"? Can I select all buffers on a stack frame?
 #reset-options "--z3rlimit 30"
 let dice_on_stack
   (st: state)
   (riot_size: riot_size_t)
-  (riot_binary: B.buffer uint8 {B.length riot_binary == v riot_size})
+  (riot_binary: B.buffer uint8{B.length riot_binary == v riot_size})
 : HST.Stack unit
   (requires fun h ->
     h `HWIface.contains` st /\
@@ -138,31 +60,44 @@ let dice_on_stack
               (Spec.Agile.Hash.hash alg (B.as_seq h0 riot_binary))))
 =
   HST.push_frame();
+
   let uds, cdi = get_uds st, get_cdi st in
 
-  (* compute digest of `uds` *)
+  (**)let h0 = HST.get () in
+
+  (* compute uDigest *)
   let uDigest: b:B.buffer uint8{B.length b == hash_length alg}
-    = B.alloca (u8 0x00) digest_length
-  in compute_uDigest uDigest uds;
+    = B.alloca (u8 0x00) digest_length in
+  dice_hash alg
+    uds uds_length
+    uDigest;
 
-  (* compute measurement of RIoT firmware *)
+  (**)let h1 = HST.get () in
+  (**)assert (B.modifies (B.loc_buffer uDigest) h0 h1 /\
+  (**)        B.as_seq h1 uDigest == Spec.Agile.Hash.hash alg (B.as_seq h0 uds));
+
+  (* compute rDigest *)
   let rDigest: b:B.buffer uint8{B.length b == hash_length alg}
-    = B.alloca (u8 0x00) digest_length
-  in compute_rDigest rDigest riot_size riot_binary;
+    = B.alloca (u8 0x00) digest_length in
+  dice_hash alg
+    riot_binary riot_size
+    rDigest;
 
-  (* compute `cdi` *)
+  (**)let h2 = HST.get () in
+  (**)assert (B.modifies (B.loc_buffer rDigest) h1 h2 /\
+  (**)        B.as_seq h2 rDigest == Spec.Agile.Hash.hash alg (B.as_seq h1 riot_binary));
+
+  (* compute cdi *)
   dice_hmac alg
     cdi
-    uDigest (hash_len alg)
-    rDigest (hash_len alg);
+    uDigest digest_length
+    rDigest digest_length;
 
   HST.pop_frame()
 
 /// <><><><><><><><><><><><> DICE main funtion <><><><><><><><><><><>
-/// DICE main function which has `ST` effect, can do heap and stack allocation
-/// It allocates and manipulates in heap using hardware interface, and computes cdi on stack using the `dice_on_stack` function.
 
-#reset-options "--z3rlimit 30"
+#reset-options "--z3rlimit 50"
 let dice_main
   (riot_size: riot_size_t)
   (riot_binary: B.buffer uint8 {B.length riot_binary == v riot_size})
@@ -173,10 +108,14 @@ let dice_main
     (let (| _, _, local_st |) = local_state in
       B.loc_disjoint (B.loc_buffer riot_binary) (B.loc_mreference local_st)))
   (ensures  fun h0 _ h1 ->
+    (*FIXME: sometimes I can prove this, sometimes not*)//B.live h1 riot_binary /\
     uds_is_disabled)
 =
   (* allocating in the heap *)
-  let st = initialize riot_binary in
+  (* pass `riot_binary` to `initialize` in order to maintain disjointness *)
+  let st: st:state{B.all_disjoint ((get_loc_l st)@[B.loc_buffer riot_binary])}
+      = initialize riot_binary in
+
 
   (* only allocating on the stack *)
   dice_on_stack st riot_size riot_binary;
@@ -185,12 +124,7 @@ let dice_main
   unset_uds st;
   disable_uds st;
 
-  (* FIXME: I failed to prove the liveness of `riot_binary` after freeing `uds` in `disable_uds`*)
-  (**)//let h = HST.get () in
-  (**)assert (B.disjoint riot_binary (get_uds st));
-  (**)//assert (B.live h riot_binary);
-
-  st
+  (*return*) st
 
 /// <><><><><><><><><><><><> C main funtion <><><><><><><><><><><>
 
@@ -201,6 +135,50 @@ assume val riot_binary:
     {B.length b == v riot_size /\
     (let (| _, _, local_st |) = local_state in
       B.loc_disjoint (B.loc_buffer b) (B.loc_mreference local_st))}
+
+assume val safe_load
+  (riot_size: riot_size_t)
+  (riot_binary: B.buffer uint8{B.length riot_binary == v riot_size})
+  (base_address: B.buffer pub_uint8)
+: HST.Stack unit
+  (requires fun h ->
+    B.live h riot_binary /\
+    B.live h base_address)
+  (ensures  fun h0 _ h1 ->
+    B.modifies (B.loc_buffer riot_binary) h0 h1)
+
+let riot_main_t =
+  (st:state)
+-> HST.Stack state
+  (requires fun h ->
+    uds_is_disabled /\
+    h `B.live` riot_binary /\
+    (let (| _, _, local_st |) = local_state in
+      B.loc_disjoint (B.loc_buffer riot_binary) (B.loc_mreference local_st)) /\
+    (let uds_value, cdi = get_uds_value st, get_cdi st in
+     B.as_seq h cdi
+        == Spec.Agile.HMAC.hmac alg
+             (Spec.Agile.Hash.hash alg uds_value)
+             (Spec.Agile.Hash.hash alg (B.as_seq h riot_binary))))
+  (ensures  fun h0 _ h1 ->
+    let cdi = get_cdi st in
+      B.as_seq h1 cdi == Seq.create (v cdi_length) (u8 0x00))
+
+assume val riot_main: riot_main_t
+
+val safe_call
+    (riot_main: riot_main_t)
+    (st: state)
+: HST.Stack (st:state{B.all_disjoint ((get_loc_l st)@[B.loc_buffer riot_binary])})
+  (requires fun h ->
+    uds_is_disabled /\
+    h `B.live` riot_binary /\
+    (let (| _, _, local_st |) = local_state in
+      B.loc_disjoint (B.loc_buffer riot_binary) (B.loc_mreference local_st)))
+  (ensures  fun h0 _ h1 ->
+    B.live h1 riot_binary /\
+    uds_is_disabled)
+let safe_call riot_main st = riot_main st
 
 let main ()
 : HST.ST C.exit_code
